finally finished proving link between the weird statement of constant-timeness and the typical statement.  integrated it into compiler_correct_wp.  Had to use lem:(

compiler/src/compiler/Pipeline.v
@@ -570,12 +570,12 @@ Section WithWordAndMem.
             initial.(getLog) = t ->
             machine_ok p_funcs stack_lo stack_hi instrs mH Rdata Rexec initial ->
             runsTo initial (fun final : MetricRiscvMachine =>
-              exists mH' retvals,
+              (exists mH' retvals,
                 arg_regs_contain (getRegs final) retvals /\
                 post final.(getLog) mH' retvals /\
                 map.only_differ initial.(getRegs) reg_class.caller_saved final.(getRegs) /\
                 final.(getPc) = ret_addr /\
-                  machine_ok p_funcs stack_lo stack_hi instrs mH' Rdata Rexec final /\
+                  machine_ok p_funcs stack_lo stack_hi instrs mH' Rdata Rexec final) /\
               exists tL F,
               final.(getTrace) = tL ++ initial.(getTrace) /\
                 forall fuel,
@@ -596,7 +596,7 @@ Section WithWordAndMem.
       specialize (C fname next).
       cbv iota in C.
       fwd. exists next'. intuition eauto 20.
-      specialize C with (1 := H1). clear H1. fwd. eauto 10.
+      specialize C with (1 := H1). clear H1. fwd. exists f_rel_pos. intuition eauto 10.
     Qed.
 
     Definition instrencode(p: list Instruction): list byte :=
@@ -646,12 +646,12 @@ Section WithWordAndMem.
         initial.(getLog) = t ->
         machine_ok p_funcs stack_lo stack_hi instrs mH Rdata Rexec initial ->
         runsTo initial (fun final : MetricRiscvMachine =>
-          exists mH' retvals,
+          (exists mH' retvals,
             arg_regs_contain (getRegs final) retvals /\
             post final.(getLog) mH' retvals /\
             map.only_differ initial.(getRegs) reg_class.caller_saved final.(getRegs) /\
             final.(getPc) = ret_addr /\
-              machine_ok p_funcs stack_lo stack_hi instrs mH' Rdata Rexec final /\
+              machine_ok p_funcs stack_lo stack_hi instrs mH' Rdata Rexec final) /\
               exists tL F,
                 final.(getTrace) = tL ++ initial.(getTrace) /\
                   forall fuel,
@@ -671,6 +671,314 @@ Section WithWordAndMem.
         unfold map.of_list_zip in *. eauto 10.
       - fwd. rewrite H3 in G. injection G as G. subst.
         eapply C; clear C; try assumption; try congruence.
+    Qed.
+
+    
+Print FlatToRiscvDef.qLeakageEvent.
+Fixpoint trace_of_predictor so_far next fuel :=
+  match fuel with
+  | O => nil
+  | S fuel' =>
+      match next fuel so_far with
+      | Some (FlatToRiscvDef.qLE e) => e :: trace_of_predictor (app so_far (cons e nil)) next fuel'
+      | Some (FlatToRiscvDef.qendLE) => []
+      | None => []
+      end
+  end.
+
+Notation predictsLE := FlatToRiscvCommon.predictsLE.
+Print FlatToRiscvDef.qLeakageEvent.
+Lemma predictsLE_end f l :
+      predictsLE f l ->
+      f l = Some FlatToRiscvDef.qendLE.
+Proof.
+  intros H. induction H.
+  - rewrite H0. assumption.
+  - assumption.
+Qed.
+
+Lemma trace_of_predictor_works' so_far next F k :
+  (forall fuel,
+    (F <= fuel)%nat ->
+    predictsLE (next fuel) (so_far ++ k)) ->
+  exists F',
+    (forall fuel,
+        (F' <= fuel)%nat ->
+        k%list = trace_of_predictor so_far next fuel).
+Proof.
+  intros H. generalize dependent so_far. subst. induction k.
+  - intros. exists (S F). intros. destruct fuel as [|fuel']; [blia|]. simpl.
+    specialize (H (S fuel') ltac:(blia)). rewrite List.app_nil_r in H.
+    apply predictsLE_end in H. rewrite H. reflexivity.
+  - intros.
+    specialize (IHk (so_far ++ [a])%list). rewrite <- app_assoc in IHk.
+    specialize (IHk H). destruct IHk as [F' IHk]. 
+    exists (S (F + F')). intros. destruct fuel as [|fuel']; [blia|].
+    specialize (H (S fuel') ltac:(blia)). Search predictsLE.
+    apply FlatToRiscvFunctions.predictLE_cons in H. simpl. rewrite H. simpl. f_equal.
+    apply IHk. blia.
+Qed.
+
+Lemma trace_of_predictor_works next F k :
+  (forall fuel,
+    (F <= fuel)%nat ->
+    predictsLE (next fuel) k) ->
+  exists F',
+    (forall fuel,
+        (F' <= fuel)%nat ->
+        k = trace_of_predictor [] next fuel).
+Proof.
+  intros. replace k with ([] ++ k)%list by reflexivity. eapply trace_of_predictor_works'.
+  apply H.
+Qed.
+
+Require Import riscv.Utility.MonadT.
+
+Lemma predictsLE_ext p1 p2 l :
+  (forall x, p1 x = p2 x) ->
+  predictsLE p1 l ->
+  predictsLE p2 l.
+Proof.
+  intros H H0. induction H0.
+  - econstructor.
+    + rewrite <- H. assumption.
+    + intros. rewrite <- H. auto.
+    + assumption.
+  - constructor. rewrite <- H. assumption.
+Qed.
+
+Lemma predictLE_unique p l1 l2 :
+  predictsLE p l1 ->
+  predictsLE p l2 ->
+  l1 = l2.
+Proof.
+  intros. generalize dependent l2. generalize dependent p. induction l1.
+  - intros. destruct l2; [reflexivity|]. remember [] as thing. destruct H; try congruence.
+    destruct H0; try congruence. rewrite H0 in H. injection H as H.
+    cbv [FlatToRiscvDef.quotLE] in H. congruence.
+  - intros. destruct l2 eqn:E.
+    + clear IHl1. remember [] as thing. destruct H; try congruence. destruct H0; try congruence.
+      rewrite H0 in H. injection H as H.
+      cbv [FlatToRiscvDef.quotLE] in H. congruence.
+    + remember (a :: l1) as l1'. destruct H.
+      -- destruct H0.
+         ++ rewrite H0 in H. injection H as H. subst. f_equal. injection Heql1'. intros. subst.
+            eapply IHl1.
+            --- exact H2.
+            --- eapply predictsLE_ext. 2: eassumption. intros. rewrite <- H3, H1. reflexivity.
+         ++ rewrite H0 in H. injection H as H. cbv [FlatToRiscvDef.quotLE] in H. congruence.
+      -- destruct H0; congruence.
+Qed.
+
+(* This should be easy to prove, though. *)
+Lemma a_trace_sorta_exists :
+  forall next,
+  exists finalTrace,
+  forall initial P,
+  FlatToRiscvCommon.runsTo initial
+    (fun final : MetricRiscvMachine =>
+       P final /\
+         (exists (tL : list LeakageEvent) (F : nat),
+             getTrace final = (tL ++ getTrace initial)%list /\
+               (forall fuel : nat,
+                   (F <= fuel)%nat ->
+                   FlatToRiscvCommon.predictsLE (next fuel)
+                     (rev tL)))) ->
+    FlatToRiscvCommon.runsTo initial
+      (fun final : MetricRiscvMachine =>
+         P final /\ exists F,
+           forall fuel : nat,
+             (F <= fuel)%nat ->
+             getTrace final = finalTrace fuel ++ getTrace initial).
+Proof.
+  intros. exists (fun fuel => (rev (trace_of_predictor nil next fuel))%list).
+  intros.
+  cbv [FlatToRiscvCommon.runsTo]. eapply runsToNonDet.runsTo_weaken.
+  1: eapply H. simpl. intros. destruct H0 as [H1 [tL [F [H2 H3] ] ] ].
+  split; [assumption|]. assert (H3' := H3).
+  apply trace_of_predictor_works in H3. destruct H3 as [F' H3].
+  intros. simpl in H. exists F'. intros. rewrite H2. f_equal.
+  rewrite <- (rev_involutive tL). f_equal. apply H3. apply H0.
+Qed.
+
+Require Import riscv.Platform.MetricSane.
+
+Print FlatToRiscvCommon.runsTo.
+Search runsToNonDet.runsTo.
+
+Print runsToNonDet.runsTo.
+
+Definition P : nat -> Prop := fun n => (n <= 5)%nat.
+
+Check run1_sane. Check (run1 _).
+Print mcomp_sane.
+Lemma runsTo_sane :
+  forall (st : MetricRiscvMachine) (post : MetricRiscvMachine -> Prop),
+    valid_machine st ->
+    FlatToRiscvCommon.runsTo st post ->
+    (exists (st' : MetricRiscvMachine), post st' /\ valid_machine st') /\
+      FlatToRiscvCommon.runsTo st
+        (fun (st' : MetricRiscvMachine) =>
+           (post st' /\ (exists diff : list LogItem, getLog st' = (diff ++ getLog st)%list)) /\
+             valid_machine st').
+Proof.
+  intros. induction H0.
+  - split.
+    + exists initial. split; assumption.
+    + constructor. split; [|assumption]. split; [assumption|]. exists nil. reflexivity.
+  - assert (H3 := run1_sane iset). cbv [mcomp_sane] in H3.
+    specialize (H3 initial (fun _ => midset) H H0).
+    destruct H3 as [ [_ [midst [H3 H4] ] ] H5].
+    split.
+    + specialize (H2 midst H3 H4). destruct H2 as [H2 H2'].  exact H2.
+    + Print runsToNonDet.runsTo. eapply runsToNonDet.runsToStep.
+      -- exact H5.
+      -- simpl. intros mid [ [H6 H7] H8]. specialize (H2 mid H6 H8).
+         destruct H2 as [_ H2]. eapply runsToNonDet.runsTo_weaken.
+         ++ exact H2.
+         ++ simpl. intros final [ [H9 [diff H10] ] H11].
+            split; [|assumption]. split; [assumption|]. rewrite H10.
+            destruct H7 as [diff' H7]. rewrite H7. eexists. rewrite <- app_assoc. reflexivity.
+Qed.
+
+Lemma last_step_useless_version :
+  forall
+    (finalTrace : nat -> list LeakageEvent)
+    (initial : MetricRiscvMachine)
+    (P : MetricRiscvMachine -> Prop),
+    valid_machine initial ->
+    
+    FlatToRiscvCommon.runsTo initial
+      (fun final : MetricRiscvMachine =>
+         P final /\
+           exists F,
+           forall fuel : nat,
+             (F <= fuel)%nat ->
+             getTrace final = finalTrace fuel ++ getTrace initial) ->
+
+    exists n,
+    FlatToRiscvCommon.runsTo initial
+      (fun final : MetricRiscvMachine =>
+         P final /\
+           getTrace final = finalTrace n ++ getTrace initial).
+Proof. Abort.
+
+Axiom em : forall P, P \/ ~P. 
+
+Lemma last_step :
+  forall (finalTrace : nat -> list LeakageEvent),
+    
+  exists (n : nat),
+  forall (initial : MetricRiscvMachine)
+         (P : MetricRiscvMachine -> Prop),
+    valid_machine initial ->
+    
+    FlatToRiscvCommon.runsTo initial
+      (fun final : MetricRiscvMachine =>
+         P final /\
+           exists F,
+           forall fuel : nat,
+             (F <= fuel)%nat ->
+             getTrace final = finalTrace fuel ++ getTrace initial) ->
+    
+    FlatToRiscvCommon.runsTo initial
+      (fun final : MetricRiscvMachine =>
+         P final /\
+           getTrace final = finalTrace n ++ getTrace initial).
+Proof.
+  intros finalTrace.
+  assert (H := em (exists F, forall fuel, (F <= fuel)%nat -> finalTrace fuel = finalTrace F)).
+  destruct H as [H|H].
+  - destruct H as [F H]. exists F. intros. eapply runsToNonDet.runsTo_weaken.
+    + eassumption.
+    + simpl. intros final [H2 [F' H3] ]. split; [assumption|].
+      specialize (H (F + F')%nat ltac:(blia)). specialize (H3 (F + F')%nat ltac:(blia)).
+      rewrite <- H. apply H3.
+  - exists O. intros. eapply runsToNonDet.runsTo_weaken.
+    + eassumption.
+    + simpl. intros. destruct H2 as [_ H2]. exfalso. apply H. destruct H2 as [F H2].
+      exists F. intros. assert (H4 := H2 F ltac:(blia)). assert (H5 := H2 fuel ltac:(blia)).
+      rewrite H4 in H5. Search (_ ++ _ = _ ++ _ -> _ = _). apply app_inv_tail in H5. symmetry.
+      assumption.
+Qed.
+
+Check a_trace_sorta_exists.
+Check last_step.
+
+Lemma predictor_thing_correct :
+  forall (next : nat -> list LeakageEvent -> option FlatToRiscvDef.qLeakageEvent),
+  exists finalTrace,
+    forall (initial : MetricRiscvMachine) (P : MetricRiscvMachine -> Prop),
+    valid_machine initial ->
+    FlatToRiscvCommon.runsTo initial
+      (fun final : MetricRiscvMachine =>
+         P final /\
+           (exists (tL : list LeakageEvent) (F : nat),
+               getTrace final = (tL ++ getTrace initial)%list /\
+                 (forall fuel : nat, (F <= fuel)%nat -> predictsLE (next fuel) (rev tL)))) ->
+      FlatToRiscvCommon.runsTo initial
+        (fun final : MetricRiscvMachine => P final /\ getTrace final = finalTrace ++ getTrace initial).
+Proof.
+  intros next.
+  assert (H := a_trace_sorta_exists next).
+  destruct H as [finalTrace H].
+  assert (H' := last_step finalTrace).
+  destruct H' as [n H'].
+  exists (finalTrace n). intros initial P H1 H2.
+  specialize (H initial P). specialize (H' initial P H1). apply H'. apply H. auto 20.
+Qed.
+
+    Lemma compiler_correct_wp': forall
+        (* input of compilation: *)
+        (fs: list (string * (list string * list string * cmd)))
+        (* output of compilation: *)
+        (instrs: list Instruction) (finfo: list (string * Z)) (req_stack_size: Z)
+        (* function we choose to call: *)
+        (stack_lo stack_hi ret_addr p_funcs: word)
+        (fname: string) next (f_rel_pos: Z),
+        (*can i move these three hyps down below the exists?*)
+        valid_src_funs fs = true ->
+        compile fs = Success (instrs, finfo, req_stack_size) ->
+        exists finalTrace, forall
+        (* high-level initial state & post on final state: *)
+        (k: trace) (t: io_trace) (mH: mem) (argvals: list word) (post: io_trace -> mem -> list word -> Prop) (initial: MetricRiscvMachine)
+        (* ghost vars that help describe the low-level machine: *)
+        (Rdata Rexec: mem -> Prop),
+        NoDup (map fst fs) ->
+        WeakestPrecondition.call fs fname k t mH argvals
+          (fun k' t' m' rets =>
+             post t' m' rets /\
+               exists k'' F,
+                 k' = k'' ++ k /\
+                   forall fuel,
+                     le F fuel ->
+                     predicts (next tt fuel) (rev k'')) ->
+        map.get (map.of_list finfo) fname = Some f_rel_pos ->
+        req_stack_size <= word.unsigned (word.sub stack_hi stack_lo) / bytes_per_word ->
+        word.unsigned (word.sub stack_hi stack_lo) mod bytes_per_word = 0 ->
+        initial.(getPc) = word.add p_funcs (word.of_Z f_rel_pos) ->
+        map.get (getRegs initial) RegisterNames.ra = Some ret_addr ->
+        word.unsigned ret_addr mod 4 = 0 ->
+        arg_regs_contain initial.(getRegs) argvals ->
+        initial.(getLog) = t ->
+        machine_ok p_funcs stack_lo stack_hi instrs mH Rdata Rexec initial ->
+        FlatToRiscvCommon.runsTo initial (fun final : MetricRiscvMachine =>
+          (exists mH' retvals,
+            arg_regs_contain (getRegs final) retvals /\
+            post final.(getLog) mH' retvals /\
+            map.only_differ initial.(getRegs) reg_class.caller_saved final.(getRegs) /\
+            final.(getPc) = ret_addr /\
+              machine_ok p_funcs stack_lo stack_hi instrs mH' Rdata Rexec final) /\
+              final.(getTrace) = finalTrace ++ initial.(getTrace)).
+    Proof.
+      intros. Check compiler_correct_wp.
+      assert (H' := compiler_correct_wp fs instrs finfo req_stack_size fname next f_rel_pos ltac:(assumption) ltac:(assumption)).
+      destruct H' as [next' H']. Check predictor_thing_correct.
+      assert (H'' := predictor_thing_correct (next' (p_funcs, f_rel_pos, stack_hi))).
+      destruct H'' as [finalTrace H''].
+      exists finalTrace. intros. apply H''.
+      - destruct H11 as (H11_1 & H11_2 & H11_3 & H11_4 & H11_5 & H11_6 & H11_7). assumption.
+      - eapply H'; eassumption.
     Qed.
 
   End WithMoreParams.
